finish simple parallel add

theories/coneris/examples/parallel_add.v
@@ -1,6 +1,39 @@
-From clutch.coneris Require Import coneris par lib.flip.
+From iris.algebra Require Import excl_auth.
+From iris.base_logic.lib Require Import invariants.
+From clutch.coneris Require Import coneris par spawn lib.flip.
 
 Local Open Scope Z.
+
+Set Default Proof Using "Type*".
+
+Section lemmas.
+  Context `{!inG Σ (excl_authR boolO)}.
+
+  (* Helpful lemmas *)
+  Lemma ghost_var_alloc b :
+    ⊢ |==> ∃ γ, own γ (●E b) ∗ own γ (◯E b).
+  Proof.
+    iMod (own_alloc (●E b ⋅ ◯E b)) as (γ) "[??]".
+    - by apply excl_auth_valid.
+    - by eauto with iFrame.
+  Qed.
+
+  Lemma ghost_var_agree γ b c :
+    own γ (●E b) -∗ own γ (◯E c) -∗ ⌜ b = c ⌝.
+  Proof.
+    iIntros "Hγ● Hγ◯".
+    by iCombine "Hγ● Hγ◯" gives %<-%excl_auth_agree_L.
+  Qed.
+
+  Lemma ghost_var_update γ b' b c :
+    own γ (●E b) -∗ own γ (◯E c) ==∗ own γ (●E b') ∗ own γ (◯E b').
+  Proof.
+    iIntros "Hγ● Hγ◯".
+    iMod (own_update_2 _ _ _ (●E b' ⋅ ◯E b') with "Hγ● Hγ◯") as "[$$]".
+    { by apply excl_auth_update. }
+    done.
+  Qed.
+End lemmas.
 
 Section simple_parallel_add.
 Definition simple_parallel_add : expr :=
@@ -11,6 +44,71 @@ Definition simple_parallel_add : expr :=
   ;;
   !"r".
 
+(* Simple spec, where the error is directly distributed *)
+Context `{!conerisGS Σ, !spawnG Σ, !inG Σ (excl_authR boolO)}.
+
+Definition simple_parallel_add_inv (l:loc) (γ1 γ2 : gname) : iProp Σ :=
+  ∃ (b1 b2 : bool) (z : Z),
+      own γ1 (●E b1) ∗ own γ2 (●E b2) ∗ l ↦ #z ∗
+      ⌜(z = bool_to_Z b1 + bool_to_Z b2)%Z⌝.
+
+
+Lemma simple_parallel_add_spec:
+  {{{ ↯ (2/3) }}}
+    simple_parallel_add
+    {{{ (z:Z), RET #z; ⌜(z=2)⌝ }}}.
+Proof.
+  iIntros (Φ) "Herr HΦ".
+  rewrite /simple_parallel_add.
+  wp_alloc l as "Hl".
+  wp_pures.
+  iMod (ghost_var_alloc false) as (γ1) "[Hγ1● Hγ1◯]".
+  iMod (ghost_var_alloc false) as (γ2) "[Hγ2● Hγ2◯]".
+  iMod (inv_alloc nroot _ (simple_parallel_add_inv l γ1 γ2) with "[Hl Hγ1● Hγ2●]") as "#I".
+  { iModIntro. iExists _, _, _. iFrame. iPureIntro. simpl. lia. }
+  replace (2/3)%R with (/3 + /3)%R by lra.
+  iDestruct (ec_split with "[$]") as "[Herr1 Herr2]"; [lra|lra|].
+  wp_apply (wp_par (λ _, own γ1 (◯E true))%I (λ _, own γ2 (◯E true))%I
+             with "[Herr1 Hγ1◯][Herr2 Hγ2◯]").
+  { wp_apply (wp_rand_err_nat _ _ 0%nat).
+    replace (INR (Z.to_nat 2) + 1)%R with 3%R; [iFrame|simpl; lra].
+    iIntros (??).
+    wp_pures.
+    rewrite bool_decide_eq_true_2; last lia.
+    wp_pures.
+    iInv "I" as (???) ">(Hγ1● & Hγ2● & Hl & %)" "Hclose".
+    iDestruct (ghost_var_agree with "[$Hγ1●][$]") as "->".
+    wp_faa.
+    iMod (ghost_var_update _ true with "[$Hγ1●][$]") as "[Hγ1● Hγ1◯]".
+    iMod ("Hclose" with "[Hγ1● Hγ2● Hl]"); last done.
+    iModIntro. iExists _, _, _. iFrame.
+    iPureIntro. simpl in *. lia.
+  }
+  { wp_apply (wp_rand_err_nat _ _ 0%nat).
+    replace (INR (Z.to_nat 2) + 1)%R with 3%R; [iFrame|simpl; lra].
+    iIntros (??).
+    wp_pures.
+    rewrite bool_decide_eq_true_2; last lia.
+    wp_pures.
+    iInv "I" as (???) ">(Hγ1● & Hγ2● & Hl & %)" "Hclose".
+    iDestruct (ghost_var_agree with "[$Hγ2●][$]") as "->".
+    wp_faa.
+    iMod (ghost_var_update _ true with "[$Hγ2●][$]") as "[Hγ2● Hγ2◯]".
+    iMod ("Hclose" with "[Hγ1● Hγ2● Hl]"); last done.
+    iModIntro. iExists _, _, _. iFrame.
+    iPureIntro. simpl in *. lia.
+  }
+  iIntros (??) "[??]".
+  iNext. wp_pures.
+  iInv "I" as (???) ">(Hγ1● & Hγ2● & Hl & %)" "Hclose".
+  iDestruct (ghost_var_agree with "[$Hγ1●][$]") as "->".
+  iDestruct (ghost_var_agree with "[$Hγ2●][$]") as "->".
+  simpl in *. subst. wp_load.
+  iMod ("Hclose" with "[Hγ1● Hγ2● Hl]").
+  - iNext. by iFrame.
+  - iApply "HΦ". iPureIntro. lia.
+Qed. 
+
 End simple_parallel_add.
 
 Section parallel_add.
@@ -19,7 +117,7 @@ Definition parallel_add : expr :=
   let: "r" := ref #0 in
   ( if: flip then FAA "r" #1 else #())
   |||
-  (if: #0 < rand #2 then FAA "r" #1 else #())
+  (if: flip then FAA "r" #1 else #())
   ;;
   !"r".
 
